lazy_list/inv.v
@@ -1,0 +1,125 @@
+From Coq Require Import Sorting.Sorted.
+
+From iris.heap_lang Require Import proofmode.
+From iris.base_logic.lib Require Import invariants.
+
+From SkipList.lib Require Export lemmas.
+
+
+Local Open Scope Z.
+Module LazyListInv (Params: LAZY_LIST_PARAMS).
+  Import Params.
+  Module Lemmas := LazyListLemmas Params.
+  Import Lemmas.
+
+  Section Proofs.
+    Context `{!heapGS Σ} (N : namespace).
+    
+    (* 
+    * The invariant for the lazy list asserts that
+    * there exists an abstract list L equivalent to 
+    * the in-memory list. The underlying list L is 
+    * sorted and must contain the same elements as 
+    * the abstract set S.
+    *)
+
+    Fixpoint list_equiv (L: list node_rep) : iProp Σ :=
+      match L with
+      | nil => True
+      | pred :: succs => 
+        match succs with
+        | nil => ∃ (l: loc), 
+                 ⌜ node_next pred = Some l ⌝
+                 ∗
+                 l ↦ rep_to_node tail
+
+        | succ :: t => ∃ (l: loc), 
+                       ⌜ node_next pred = Some l ⌝
+                       ∗
+                       l ↦ rep_to_node succ
+                       ∗
+                       list_equiv succs
+        end
+      end.
+
+    Definition lazy_list_inv (S: gset node_rep) (head: node_rep) : iProp Σ := 
+      ∃ (L: list node_rep),
+      ⌜ Permutation L (elements S) ⌝
+      ∗
+      ⌜ Sorted node_lt ([head] ++ L ++ [tail]) ⌝
+      ∗
+      list_equiv ([head] ++ L)
+    .
+
+    Definition is_lazy_list (Skeys: gset Z) (head: node_rep) : iProp Σ := 
+      ∃ (S: gset node_rep),
+      ⌜ key_equiv S Skeys ⌝
+      ∗
+      ⌜ node_key head = INT_MIN ⌝
+      ∗
+      inv N (lazy_list_inv S head).
+    
+
+    Lemma list_equiv_cons (rep: node_rep) (L: list node_rep) :
+      list_equiv (rep :: L)
+        ⊢ (list_equiv L ∗ (list_equiv L -∗ list_equiv (rep :: L)))
+    .
+    Proof.
+      destruct L as [|n].
+      * iIntros "Hrep". by iFrame.
+      * iIntros "Hlist". iDestruct "Hlist" as (l) "(Hsome & Hpt & Hmatch)".
+        iFrame. iIntros "Hlist". iFrame.
+        iExists l. iFrame.
+    Qed.
+
+    Lemma list_equiv_split (pred succ: node_rep) (L L1 L2: list node_rep):
+      L ++ [tail] = L1 ++ [pred; succ] ++ L2 →
+      list_equiv L ⊢ ∃ (l: loc),
+                       ⌜ node_next pred = Some l ⌝
+                       ∗
+                       l ↦ (rep_to_node succ)
+                       ∗
+                       (l ↦ (rep_to_node succ) -∗ list_equiv L)
+    .
+    Proof.
+      revert L. induction L1 => L HL.
+      + destruct L as [|curr L].
+        { exfalso. inversion HL. }
+        inversion HL as [[H0 HL']]; subst.
+        destruct L as [|curr L].
+        - inversion HL'; subst.
+          iIntros "Hlist". 
+          iDestruct "Hlist" as (l) "(#Hsome & Hpt)".
+          iExists l. iFrame "#"; iFrame.
+          iIntros "Hpt". 
+          iExists l. iFrame "#"; iFrame.
+        - inversion HL'; subst.
+          iIntros "Hlist". 
+          iDestruct "Hlist" as (l) "(#Hsome & Hpt & Hmatch)".
+          iExists l. iFrame "#"; iFrame.
+          iIntros "Hpt". 
+          iExists l. iFrame "#"; iFrame.
+      + destruct L as [|curr L].
+        { 
+          exfalso. inversion HL  as [[H0 HL']]; subst. 
+          destruct L1; inversion HL'.
+        }
+        inversion HL as [[H0 HL']]; subst.
+
+        destruct L as [|curr L].
+        { 
+          exfalso. 
+          destruct L1; inversion HL. 
+          destruct L1; inversion HL.
+        }
+        
+        iIntros "Hlist".
+        iPoseProof (list_equiv_cons with "Hlist") as "(Hlist & Himp)".
+        iPoseProof (IHL1 with "Hlist") as "Hlist"; auto.
+        iDestruct "Hlist" as (l) "(Hsome & Hpt & Himp')".
+        iExists l. iFrame. iIntros "Hpt".
+        iApply "Himp". iApply "Himp'". iFrame.
+    Qed.
+
+  End Proofs.
+End LazyListInv.
